finish custom_simp

CustomSimpRw.lean
@@ -1,6 +1,11 @@
 import Batteries
 import Lean
 import Qq
+import TutorialAux.Tag -- for Section (6)
+
+/-!
+This file explains and implements basic versions of `rw` & `simp` tactics.
+-/
 
 open Lean Elab Meta Tactic
 open Qq
@@ -15,11 +20,10 @@ Content
 (4) Implementing `simp`.
 (5) Unification - rewriting a quantified equality.
 (6) Collecting tagged lemmas
-(7) Simplification procedures - building upon existing simp infrastructure
 
-Leave for another file
-* Options for `whnf`
-* Options for unification
+Left for another file
+* Normalization details
+* Unification details
 -/
 
 /-
@@ -93,7 +97,7 @@ def weirdNat : (fun t _ => t) Nat 8 := 4
 Simp doesn't do all its equal rewrites in one go.
 Instead, it recursively dives into the term, and when
 it combines two branches in which both terms got
-updated, it directly uses
+updated, it uses
 -/
 #check congr
 
@@ -106,7 +110,7 @@ theorem simp_example (a b c : Nat) (f : Nat → Nat) (p : Nat → Prop)
 #print simp_example
 
 /-
-After prettification, you could get the following proof term.
+This is muc hmore messy but after prettification, you could get the following proof term.
 -/
 example (a b c : Nat) (f : Nat → Nat) (p : Nat → Prop)
     (h_eq  : ∀ x : Nat, f x = x) (h_finish : p (a + c + b + c + a + c)) :
@@ -130,7 +134,7 @@ example (a b c : Nat) (f : Nat → Nat) (p : Nat → Prop)
   )
   h_finish
 /-
-It is not as clean as with `rw`, but you can notice that
+You can notice that
 * The expression is build gradually, not in one go.
 * We actually run `h_eq a` twice in the proof term, because
   we are rewriting with it on two places, contrary to `rw`.
@@ -185,6 +189,7 @@ A `bvar` is a variable pointing to a quantifier with an index
 where quantifiers are indexed from the inner-most to the outer-most.
 To know the index for the `bvar`, we carry `offset`.
 -/
+/-- (tutorial function) simplified `kabstract` -/
 def myAbstract (e a : Expr) (offset : Nat := 0) : MetaM Expr := do
   if !e.hasLooseBVars then  -- we cannot rewrite a subterm containing a variable bound in `e`
     if (← isDefEq e a) then  -- check if already `a` is already the root
@@ -201,10 +206,11 @@ def myAbstract (e a : Expr) (offset : Nat := 0) : MetaM Expr := do
   | .forallE _ d b _ => return e.updateForallE! (← myAbstract d a offset) (← myAbstract b a (offset+1))
   | e                => return e
 
--- lean implements this with a slightly more advanced but still readable
+-- lean's implementation is slightly more advanced but still readable
 #check kabstract
 
 -- Now, we can build the mapping
+/-- (tutorial function) Wraps the result of `kabstract` to a lambda. -/
 def abstractToMapping (e a : Expr) : MetaM Expr := do
   -- make sure that all previous mvar assignments were applied in `e`
   -- this is necessary to recurse the term, not for `isDefEq`, so `a` doesn't need it
@@ -233,13 +239,15 @@ example (A : Nat) (h : -- some crazy expression containing various constructions
 /-
 ## Decomposing equality
 -/
-/--
+/-- (tutorial function)
 `decomposeEq` takes a proof of equality `pf : a = b`, where `(a b : α : Sort u)`,
 and returns (u, α, a b)
 -/
 def decomposeEq (pf : Expr) : MetaM (Level × Expr × Expr × Expr) := do
   let t ← inferType pf
-  let t ← whnf t -- helps to get `Eq` at the root, removing mdata, instantiating mvars...
+  -- `whnf` helps to get `Eq` at the root, removing mdata,
+  -- instantiating mvars, expanding definitions...
+  let t ← whnf t
   match t with
   | .app (.app (.app (.const ``Eq [u]) α) a) b =>
     return (u, α, a, b)
@@ -250,16 +258,19 @@ def decomposeEq (pf : Expr) : MetaM (Level × Expr × Expr × Expr) := do
 
 /-
 ## Building proof term
+-/
 
-Now, we write a function that takes an equation
-a term `t := ... A ...`, and an equation `eq : A = B`,
-and returns a proof of `... B ... → ... A ...`.
+/--
+(tutorial function)
+Takes a term `t := ... A ...`, and an equation
+`eq : A = B`, and returns a proof of `... B ... → ... A ...`.
 -/
 def proveRwImp (eq t : Expr) :
   MetaM Expr := do
   let (u, α, a, b) ← decomposeEq eq
   -- find the abstract function
   let f ← abstractToMapping t a
+  logInfo m!"lhs := {a}, rhs := {b}\nabstr := {f}"
   -- we also detect the sort level of t (usually Prop)
   let tt ← inferType t
   let v := (← inferType tt).sortLevel!
@@ -308,9 +319,9 @@ example (a b : Nat) (h : a = b) : 2*a + b = 2*b + a := by
 # (3) Filling implicit arguments.
 
 When we were applying `congrArg` and `Eq.mpr`, we were explicitly filling
-the universe levels, and implicit argument. With `simp`, we will need to
-build much more terms, so let us look at the options we have with the example
-of transitivity.
+the universe levels, and implicit argument. Already there, it was a bit annoying,
+and with `simp`, we will need to build much more terms. Fortunatelly, there are
+ways to avoid this work.
 -/
 example (a b c : Nat) (pf1 : a = b) (pf2 : b = c) : True := by
   -- we would like to emulate calling something like
@@ -322,7 +333,7 @@ example (a b c : Nat) (pf1 : a = b) (pf2 : b = c) : True := by
     -- (a) low-level constructing the term, we have to provide all the arguments
     let lowlev := mkApp6 ((mkConst ``Eq.trans [1])) (mkConst ``Nat) a b c pf1 pf2
     logInfo m!"lowlev = {lowlev}"
-    -- (b) using `Qq`, the type annotation is optional
+    -- (b) using `Qq`
     let pfQ : Q($a = $c) := q(Eq.trans $pf1 $pf2)
     logInfo m!"pfq = {pfQ}"
     -- (c) using `mkAppM`
@@ -356,8 +367,8 @@ Even if these arguments are passed implicitly (so the meta-programmer doesn't
 have to write them), they are indeed passed, and play a crucial role in runtime
 to build the resulting term.
 
-Here, we will use `mkAppM` to finish the implementation of `simp`.
-Using `Qq` would require taking care of the annotations which can become
+We will use `mkAppM` to finish the implementation of `simp`.
+Using `Qq` requires taking care of the annotations which can become
 a bit finicky (doable but perhaps not as well suited for a tutorial).
 On the other hand, we encourage you to try building terms with `Qq` too,
 and see what suits your needs better.
@@ -379,8 +390,8 @@ structure SimpResult where
   expr : Expr
   pf? : Option Expr
 
--- Note that the library Simp also has a similar Result structure, both
--- in basic library, and with Qq hints, we will not use that for now
+-- Note that the library Simp also has very similar Result structure, both
+-- in basic library, and with Qq hints.
 #check Simp.Result
 #check Simp.ResultQ
 
@@ -389,7 +400,8 @@ structure SimpResult where
 def SimpResult.empty (e : Expr) : SimpResult := {expr := e, pf? := none}
 
 #check Eq.refl
-/-- Gets the proof, possibly building `rfl` if it was none. -/
+/-- (tutorial function)
+Gets the proof, possibly building `rfl` if it was none. -/
 def SimpResult.getProof (r : SimpResult) : MetaM Expr :=
   match r.pf? with
   | some pf => pure pf
@@ -397,7 +409,8 @@ def SimpResult.getProof (r : SimpResult) : MetaM Expr :=
 -- see also `mkEqRefl`
 
 #check Eq.trans
-/-- Combines two `SimpResults` using `Eq.trans` -/
+/-- (tutorial function)
+Combines two `SimpResults` using `Eq.trans` -/
 def SimpResult.trans (r1 r2 : SimpResult) : MetaM SimpResult := do
   match r1.pf? with
   | none => return r2
@@ -410,7 +423,8 @@ def SimpResult.trans (r1 r2 : SimpResult) : MetaM SimpResult := do
 #check congr
 #check congrArg
 #check congrFun
-/-- Combines `f = g`, and `a = b` into `f a = g b` using `congr` -/
+/-- (tutorial function)
+Combines `f = g`, and `a = b` into `f a = g b` using `congr` -/
 def SimpResult.app (rf rArg : SimpResult) : MetaM SimpResult := do
   let expr := mkApp rf.expr rArg.expr
   match rf.pf? with
@@ -423,7 +437,8 @@ def SimpResult.app (rf rArg : SimpResult) : MetaM SimpResult := do
 -- see also `mkCongr`, `mkCongrArg`, `mkCongrFun`
 
 #check implies_congr
-/-- from `a = b`, `c = d` proves `a → c = b → d` using `implies_congr` on `SimpResult`s -/
+/-- (tutorial function)
+from `a = b`, `c = d` proves `a → c = b → d` using `implies_congr` on `SimpResult`s -/
 def SimpResult.impl (r1 r2 : SimpResult) : MetaM SimpResult := do
   let expr := mkForall Name.anonymous BinderInfo.default r1.expr r2.expr
   if r1.pf?.isNone && r2.pf?.isNone then return .empty expr
@@ -433,7 +448,7 @@ def SimpResult.impl (r1 r2 : SimpResult) : MetaM SimpResult := do
 -- see also `mkImpCongr`
 
 #check forall_congr
-/--
+/-- (tutorial function)
 Gets a proof of `p fv = q fv` where `fv` is a free variable, and `p fv` is a `Prop`.
 and builds a proof of `(∀ x, p x) = (∀ x, q x)` using forall_congr.
 -/
@@ -451,7 +466,7 @@ def SimpResult.forall (fv : Expr) (r : SimpResult) :
 /-
 ## Main functions `SimpRec` & `SimpBase`
 
-Later, we will also want to simplify quantified equations,
+Later, we will also want to simplify tagged quantified equations,
 so we split the simplification algorithm into two functions.
 
 * Function `simpBase (...) a` only tries to make a single rewrite step
@@ -462,8 +477,8 @@ so we split the simplification algorithm into two functions.
   the term, and returns the proof of equality in the same format.
 -/
 
-/--
-This is the main simple root-rewriting function.
+/-- (tutorial function)
+Simple root-rewriting function.
 It gets a list of equalities `rules`, and tries to find a rule
 `rule : e = b` that exactly matches the given expression `e`.
 It doesn't dig inside `e`, and only tries to perform the step once.
@@ -477,6 +492,9 @@ def simpBase (rules : List Expr) (a : Expr) :
       return {expr := br, pf? := some rule}
   return .empty a
 
+/-- (tutorial function)
+Recursive rewrite inside a term.
+-/
 partial -- simplification could repeat indefinitely, `partial` skips termination check
 def simpRec (base : Expr →  MetaM SimpResult)
   (a : Expr) : MetaM SimpResult := do
@@ -514,22 +532,30 @@ def simpRec (base : Expr →  MetaM SimpResult)
   let resRepeat ← simpRec base res.expr
   res.trans resRepeat
 
--- Let's finally try it out!
-example (a b c : Nat) (p : Nat → Nat → Prop)
-    (h₁ : a = b) (h₂ : b = c) (finish : ∀ x, p x c → p x c) :
-    (∀ x, p x a → p x a) := by
-  -- simp only [h₁, h₂]
-  run_tacq goal =>
-    let res ← simpRec (simpBase [h₁, h₂]) goal.ty
+/--
+(tutorial function)
+-/
+def mySimpGoal (base : Expr → MetaM SimpResult) : TacticM Unit := do
+  let goal ← getMainGoal
+  goal.withContext do
+    let target ← goal.getType
+    let res ← simpRec base target
     logInfo m!"Simplified to {res.expr}"
     match res.pf? with
-    | none => throwError "Simplification made no progress"
+    | none => throwError "mySimpGoal made no progress"
     | some pf =>
       logInfo m!"proof of equality: {pf}"
       -- use Eq.mpr as before, this time using `mkAppM`
       let m ← mkFreshExprSyntheticOpaqueMVar res.expr
-      goal.mvarId!.assign <| ← mkAppM ``Eq.mpr #[pf, m]
+      goal.assign <| ← mkAppM ``Eq.mpr #[pf, m]
       replaceMainGoal [m.mvarId!]
+
+-- Test!
+example (a b c : Nat) (p : Nat → Nat → Prop)
+    (h₁ : a = b) (h₂ : b = c) (finish : ∀ x, p x c → p x c) :
+    (∀ x, p x a → p x a) := by
+  -- simp only [h₁, h₂]
+  run_tacq mySimpGoal (simpBase [h₁, h₂])
   exact finish
 
 /-
@@ -540,20 +566,24 @@ we don't have to implement the entire `simpRec` from scratch. Let us show how
 to perform the same simplification using our own `simpBase` but library's `simp`.
 -/
 
+#print Simp.Simproc
+#check Simp.main
+#check applySimpResultToTarget
+
 example (a b c : Nat) (p : Nat → Nat → Prop)
     (h₁ : a = b) (h₂ : b = c) (finish : ∀ x, p x c → p x c) :
     (∀ x, p x a → p x a) := by
   -- simp only [h₁, h₂]
   run_tacq goal =>
-    let ctx : Simp.Context ← Simp.mkContext -- optional lemmas & extra congruence lemmas
-    let methods : Simp.Methods := { pre := fun e => do
+    let ctx : Simp.Context ← Simp.mkContext -- optionally lemmas & extra congruence lemmas
+    let method : Simp.Simproc := fun e : Expr => do
       let res ← simpBase [h₁, h₂] e
       -- Very straightforward translation from our `SimpResult` to the library
       -- `Simp.Step`. In general, `Simp.Step` can guard the repetition inside
-      -- inside `simp` by deciding on `done` / `visit` / `continue`
+      -- `simp` by deciding on `done` / `visit` / `continue`
       if res.pf?.isNone then return Simp.Step.continue
       else return Simp.Step.visit { expr := res.expr, proof? := res.pf? }
-    }
+    let methods : Simp.Methods := { pre := method }
     let (res, _stats) ← Simp.main goal.ty ctx (methods := methods)
     logInfo m!"Simplified to {res.expr}"
     -- we could match on `res.proof?` as above but we can also use library function
@@ -564,34 +594,158 @@ example (a b c : Nat) (p : Nat → Nat → Prop)
 
 /-
 # (5) Unification - rewriting a quantified equality.
--/
 
--- TODO:
--- basics of unification theory (first-order in almost linear time,
---   second order undecidable, but lean has some heuristics)
--- in practice
--- * replace forall with metavariables
--- * explain & run isDefEq
+Now, we want to be able to rewrite quantified equality, say we have the rule
+`∀ a b : Nat, p a + b = a + q b`,
+and we want to use it to rewrite `p 1 + 2` to `1 + q 2`.
+The main idea is to first replace the quantified variables with metavariables to obtain
+`p ?a + ?b = p ?b + ?a`
+Now the left hand side is structurally the same as `p 1 + 2` up to the
+metavariables, so we need to find the right value for them.
+
+Finding values for metavariables actually happens automatically:
+-/
+example (p : Nat → Nat) : True := by
+  run_tacq
+    let a ← mkFreshExprMVarQ q(Nat) (userName := `a) -- just a Qq-sugar on top
+    let b ← mkFreshExprMVarQ q(Nat) (userName := `b) -- of `mkFreshExprMVar`
+    let pattern := q($p $a + $b)
+    let rhs := q($a + $p $b)
+    let target := q($p 1 + 2)
+    logInfo m!"matching {target} with {pattern} → {rhs}" -- not assigned
+    if ← isDefEq pattern target then -- The magic happens here!
+      logInfo m!"matched {target} with {pattern} → {rhs}" -- assigned
+    else
+      logInfo "Couldn't match"
+    logInfo m!"If match succeesed, the mvars are now assigned: a = {a}, b = {b}"
+    -- Note that using MessageData is crucial - the expressions `a`, `b` didn't change,
+    -- only the way we look at them inside MetaM Monad.
+    logInfo s!"As a string, we still see the metavariables:\na = {a}, b = {b}"
+  trivial
+
+/-
+In fact, `isDefEq` is not just an innocent check, it can modify the proofstate
+by assiging metavariables (with some rules forbidding it, such as syntheticOpaque).
+Besides checking modulo basic reductions, it tries to find variable assignment that
+satisfies the equality. If there exist an assignment, the asignment is performed in
+the proofstate, and `isDefEq` return `true`. On the other hand, if the return value
+is `false`, we know there was no change in the proof state.
+
+Since we used `isDefEq` in `myAbstract`, it should be no surprise now why
+rewriting with a quantified equality matches its first instantiation.
+The unification happens the first moment it can, and later `f a` cannot
+get unified with `f b`.
+
+It is time to also reduce the willingness of `isDefEq` to reduce the term
+to find a match. We do it by setting the transparency:
+-/
+#check TransparencyMode.default -- expand definitions
+#check TransparencyMode.reducible -- expands only `abbrev`
+/-
+We will cover the options for unification / normalization in more detail in another
+file. Now let's finish the implementation by turning quantifiers into metavariables.
+The function to do it is `forallMetaTelescope`
+-/
+#check forallMetaTelescope
+-- rewrite a quantified equality
+example (a b : Nat) (f : Nat → Nat) (p : Nat → Prop)
+    (h_eq  : ∀ x : Nat, f x = x) (h_finish : p (a + b + a + b)) :
+    p (f a + f b + f a + f b) := by
+  run_tacq goal =>
+    let (mvars, _, eq) ← forallMetaTelescope h_eq.ty -- turn quantifiers into mvars
+    let pf_eq := mkAppN h_eq mvars -- build the proof term
+    logInfo m!"before: {pf_eq} : {eq}"
+    -- the same rewrite code as before
+    let imp ← withTransparency .reducible <| proveRwImp pf_eq goal.ty
+    logInfo m!"after: {pf_eq} : {eq}"
+    let imp_t ← inferType imp
+    logInfo m!"imp_t := {imp_t}"
+    let mt := imp_t.bindingDomain!
+    let m ← mkFreshExprSyntheticOpaqueMVar mt
+    goal.mvarId!.assign (mkApp imp m)
+    replaceMainGoal [m.mvarId!]
+  -- successfully rewritten `f a` → `a`
+  rw [h_eq b] -- let's do the second step with a simple `rw` :-)
+  trivial
 
 /-
 # (6) Collecting tagged lemmas
+
+The standard `simp` doesn't need to be given the lemmas each usage, it uses
+all the lemmas tagged with `@[simp]`. Let us show an example to introduce
+a custom attribute `my_tag`.
+
+This requires two `initialize` steps.
+* Creating an environment extension `myExt` using
+  `registerSimpleScopedEnvExtension`. This will store the array of tagged theorems.
+* Registering the attribute `my_tag` itself using `registerBuiltinAttribute`.
+
+Little annoyingly, every `initialize` must be done in another file than
+where it is tested (i.e. where we tag theorems with the attribute).
+
+Look at the file `TutorialAux/Tag.lean` where these two steps are done.
+-/
+#check myExt
+
+/-
+Since we imported this file, we can now tag some theorems with `my_tag`
 -/
 
--- TODO: look into it, understand, explain
+#check Nat.add_assoc
 
-theorem cancel_around (x : Nat) : 1 + x - 1 = x := sorry
+@[my_tag] theorem add_assoc_rev (a b c : Nat) :
+  a + (b + c) = (a + b) + c := (Nat.add_assoc a b c).symm
+@[my_tag] theorem two_mul_rev (a : Nat) : a + a = 2 * a := a.two_mul.symm
+-- even some theorems are defined without `@[my_tag]`
+theorem two_mul_rev' (a b : Nat) : (b + a) + a = b + 2 * a := by omega
+theorem two_two_four (a : Nat) : 2 * (2 * a) = 4 * a := by omega
+-- we can add the attribute later
+attribute [my_tag] two_mul_rev'
+attribute [my_tag] two_two_four
 
-attribute [simp] cancel_around
--- TODO: look at gcongr example in mathlib
-#check registerSimpleScopedEnvExtension
+-- look at the theorems stored at `customExt`
+run_meta
+  let state := myExt.getState (← getEnv)
+  for (e,t) in state do
+    logInfo m!"{e} : {t}"
 
+/-
+Now, we have all the ingredients to an alternative to `simpBase`.
+This will use tagged theorems (tagged when the is run), and allow
+quantified theorems.
+-/
+#check simpBase
+def simpWithTagged (expr : Expr) : MetaM SimpResult := do
+  let state := myExt.getState (← getEnv)
+  for (e,t) in state do
+    let (mvars, _, eq) ← forallMetaTelescope t -- turn quantifiers into mvars
+    let pf := mkAppN e mvars -- build the proof term
+    let some (_, ar, br) := eq.app3? ``Eq | throwError "Not an equality: {pf} : {eq}"
+    if ← withTransparency .reducible (isDefEq expr ar) then
+      return {expr := br, pf? := some pf}
+  return .empty expr
 
-/-- Environment extension for "generalized congruence" (`gcongr`) lemmas. -/
-abbrev GCongrLemma := Nat
+example (a : Nat) (p : Nat → Prop) (h : p (4*a + 2*a + a)) :
+    p ( (a+a+a)+a+(a+a+a) ) := by
+  run_tac mySimpGoal simpWithTagged
+  exact h
 
-initialize gcongrExt : SimpleScopedEnvExtension ((Name × Name × Array Bool) × GCongrLemma)
-    (Std.HashMap (Name × Name × Array Bool) (Array GCongrLemma)) ←
-  registerSimpleScopedEnvExtension {
-    addEntry := fun m (n, lem) => m.insert n ((m.getD n #[]).push lem)
-    initial := {}
-  }
+/-
+Exercise: Update the code for `Tag.lean` & `simpWithTagged` so that
+it can accept theorems with universe levels.
+-/
+
+#check eq_self
+attribute [my_tag] eq_self
+
+example (a : Nat) : a + a = 2 * a := by
+  run_tac mySimpGoal simpWithTagged
+  exact True.intro
+
+-- Hints:
+#check getConstInfo
+#check mkFreshLevelMVarsFor
+-- Feel free to change the type (Expr × Expr) stored in `myTag`
+-- the pair `(e,t)` might not be ideal. Also remember that the metavariables
+-- must be introduced when trying to apply a theorem, not at initialization
+-- because we want different mvar instantiations at different places.
