TutorialAux/Tag.lean
@@ -1,0 +1,35 @@
+import Lean
+open Lean Meta
+
+/--
+A custom environment extension to add a theorem name, and its type.
+We store these pairs (expr, type) in a simple Array.
+-/
+initialize myExt :
+    SimpleScopedEnvExtension (Expr × Expr) (Array (Expr × Expr)) ←
+  registerSimpleScopedEnvExtension {
+    -- add a single element to the array
+    addEntry := fun arr et => arr.push et
+    -- initially, the array is empty
+    initial := #[]
+  }
+
+/--
+Custom attribute `my_tag` adding a theorem to the `myExt`
+-/
+initialize registerBuiltinAttribute {
+  name := `my_tag
+  descr := "a custom tag"
+  -- by default, assigning an attribute runs in CoreM
+  -- but we can invoke MetaM, if we need
+  add := fun name stx kind ↦ MetaM.run' do
+    -- We assume we are only registering theorems without universe levels,
+    -- Making it work with universe levels is left as an exercise.
+    let e : Expr := mkConst name
+    let t : Expr ← inferType e
+    myExt.add (e,t) -- calling `addEntry` we defined in `myExt`
+
+    -- For simplicity, we are also omiting a sanity check. Usually
+    -- you should also check here if the tagged definition makes sense
+    -- for the particular attribute before adding it to the database.
+}
